

1) show $m(a + bX) = a + b \times m(X)$

$$M(Y) = \frac{1}{N} \sum_{i=1}^N y_i$$

$$M(Y) = \frac{1}{N} \sum_{i=1}^N a + bX_i$$

$$N(M(Y)) = \sum_{i=1}^N a + \sum_{i=1}^N bX_i$$

$$N(M(Y)) = Na + b \sum_{i=1}^N X_i$$

$$M(Y) = \frac{N}{N} a + b \frac{1}{N} \sum_{i=1}^N X_i$$

$$M(Y) = a + bM(X)$$

$$M(a + bX) = a + b \times M(X)$$

2) show that $\text{cov}(X, X) = S^2$

$$\text{cov}(X, X) = \frac{1}{N} \sum_{i=1}^N (X_i - M(X))(X_i - M(X))$$

$$\text{cov}(X, X) = \frac{1}{N} \sum_{i=1}^N (X_i - M(X))^2$$

$$\text{cov}(X, X) = S^2$$

3) show that $\text{cov}(X, a + bY) = b \times \text{cov}(X, Y)$

$$\text{cov}(X, a + bY) = \frac{1}{N} \sum_{i=1}^N (X_i - M(X))((a + bY_i) - m(a + bY))$$

$$\text{cov}(X, a + bY) = \frac{1}{N} \sum_{i=1}^N (X_i - M(X))(a + bY_i - a - bM(Y))$$

$$= \frac{1}{N} \sum_{i=1}^N (X_i - M(X))(b(Y_i - M(Y)))$$

$$= b \left(\frac{1}{N} \sum_{i=1}^N (X_i - M(X))(Y_i - M(Y)) \right)$$

$$= b \text{cov}(X, Y)$$

4) show that $\text{cov}(a + bX, a + bY) = b^2 \text{cov}(X, Y)$

From part 3 we know that

$$b \text{cov}(a + bX, Y) = b(b \text{cov}(X, Y))$$

$$\text{cov}(a + bX, a + bY) = b^2 \text{cov}(X, Y)$$

5) Suppose $b > 0$ and median of X be $\text{med}(X)$. Is it true the median of $a + bX$ is equal to $a + b \times \text{med}(X)$? Is the IQR of $a + bX$ equal to $a + b \times \text{IQR}(X)$?

As $b > 0$, order is maintained in the $X \rightarrow a + bX$ transformation. Thus, the "middle" maintains its position as middle after transformation.

$$\text{med}(a + bX) = a + b \text{med}(X)$$

↓
all values are
scaled by b and
shifted by a
then the median
is taken

↓ The median is
taken, scaled by
 b then shifted
by a

$$y = a + bx \text{ where } b > 0$$

$$Q_1(Y) = a + bQ_1(X), Q_3(Y) = a + bQ_3(X)$$

$$IQR(Y) = a + bQ_3(X) - a - bQ_1(X)$$

$$IQR(Y) = b(Q_3(X) - Q_1(X))$$

$$IQR(a + bx) = b(IQR(X))$$

$$\text{Thus } IQR(a + bx) = a + b(IQR(X))$$

$$\text{when } a = 0$$

6) Show by example that the means of x^2
and \sqrt{x} are generally not $(m(x))^2$ and $\sqrt{m(x)}$.

$$x^2$$

$$X = \{0, 1, 2\}$$

$$\text{mean of } x^2 = \frac{0^2 + 1^2 + 2^2}{3} = \frac{5}{3}$$

$$\text{mean of } x = \frac{0 + 1 + 2}{3} = 1$$

$$(m(x))^2 = 1^2 = 1$$

$$1 \neq \frac{5}{3} \text{ by counterexample, } m(x^2) \neq (m(x))^2$$

$$\sqrt{x} \quad x = \{0, 1, 4\}$$

$$\text{mean of } \sqrt{x} = \frac{\sqrt{0} + \sqrt{1} + \sqrt{4}}{3} = \frac{3}{3} = 1$$

$$\text{mean of } x = \frac{0 + 1 + 4}{3} = \frac{5}{3}$$

$$\sqrt{m(x)} = \sqrt{5/3} \quad \text{by counterexample}$$

$$m(\sqrt{x}) \neq \sqrt{m(x)}$$